Clean up some more files, update debug script file

icing/icing_testScript.sml
@@ -1,28 +1,31 @@
-(*
-  First test of Icing infrastructure
-*)
-(* CakeML *)
-open compilerTheory;
-(* FloVer *)
+(**
+  Icing benchmark input file
+  Use this file to run a CakeML AST through the Icing optimizer
+**)
+
+(* INCLUDES, do not change those *)
+open compilerTheory fromSexpTheory cfTacticsLib;
 open RealIntervalInferenceTheory ErrorIntervalInferenceTheory CertificateCheckerTheory;
-(* Icing *)
-open source_to_sourceTheory CakeMLtoFloVerTheory CakeMLtoFloVerLemsTheory;
-(* HOL libs *)
+open source_to_sourceTheory CakeMLtoFloVerTheory;
 open machine_ieeeTheory binary_ieeeTheory realTheory realLib RealArith;
-open preamble;
+open preamble astToSexprLib;
 
-val _ = new_theory "icingTest";
+val _ = new_theory "icing_test";
 
+(*
+(**
+  Define the CakeML source AST as a polyML/HOL4 declaration
+**)
 Definition theAST_def:
   theAST =
   (** REPLACE AST BELOW THIS LINE **)
   Dletrec unknown_loc
-    [("doppler","",
-      Fun "u" (Fun "v" (Fun "t"
+    [("doppler","u",
+      (Fun "v" (Fun "t"
         (** Precondition **)
         (Let NONE
          (App Opapp
-          [Var (Long "RuntimeProg" (Short "assert"));
+          [Var (Long "Runtime" (Short "assert"));
            (Log And
             (Log And
             (App (FP_cmp FP_LessEqual)
@@ -73,19 +76,41 @@ Definition theAST_def:
            ))))))]
 End
 
+Definition theMain_def:
+  theMain =
+  [Dlet unknown_loc (Pvar "it")
+   (Let (SOME "x" )
+     (App Opapp [
+        App Opapp [
+          App Opapp [
+              Var (Short "doppler");
+            App FpFromWord [Lit (Word64 4607182418800017408w)]];
+          App FpFromWord [Lit (Word64 4607182418800017408w)]];
+        App FpFromWord [Lit (Word64 4607182418800017408w)]])
+     (App Opapp [
+        Var (Long "TextIO" (Short "print"));
+        App Opapp [
+          Var (Long "Int" (Short "toString"));
+          App Opapp [
+            Var (Long "Word64" (Short "toInt"));
+            App FpToWord [Var (Short "x")]
+          ]
+        ]
+      ])
+   )]
+End
 
 (** Optimizations to be applied by Icing **)
 Definition theOpts_def:
-  theOpts =
-    <| optimisations := [
+  theOpts = extend_conf no_fp_opt_conf
+  [
       (* WRITE OPTIMISATIONS HERE AS ; SEPARATED LIST *)
        (Binop FP_Mul (Var 0) (Binop FP_Add (Var 1) (Var 2)),
        Terop FP_Fma (Var 0) (Var 1) (Var 2));
        (Binop FP_Mul (Var 0) (Binop FP_Mul (Var 1) (Var 2)),
        Binop FP_Mul (Binop FP_Mul (Var 0) (Var 1)) (Var 2))
        (* OPTIIMISATIONS END *)
-       ];
-       canOpt := T |>
+  ]
 End
 
 (** The code below stores in theorem theAST_opt the optimized version of the AST
@@ -94,12 +119,25 @@ End
 Theorem theAST_opt =
   EVAL
     (Parse.Term ‘
-      (source_to_source$compile_decs
-       theOpts [theAST])’);
+      (source_to_source$stos_pass_decs theOpts
+       [theAST])’);
+
+val fullProg =
+(EVAL
+     (Parse.Term ‘[(^(theAST_def |> concl |> rhs)); HD (^(theMain_def |> concl |> rhs))]’)
+  |> concl |> rhs);
+
+val fullOptProg =
+(EVAL
+     (Parse.Term ‘[HD (^(theAST_opt |> concl |> rhs)); HD (^(theMain_def |> concl |> rhs))]’)
+  |> concl |> rhs);
 
 Definition theProg_def:
-  theProg =
-  ^(theAST_opt |> concl |> rhs)
+  theProg = ^fullProg
+End
+
+Definition theOptProg_def:
+  theOptProg = ^fullOptProg
 End
 
 val _ = computeLib.del_funs [sptreeTheory.subspt_def];
@@ -111,20 +149,38 @@ val _ = computeLib.add_funs [realTheory.REAL_INV_1OVER,
 
 val dest_trip = (fn t => let val (t1, t2) = dest_pair t; val (t2, t3) = dest_pair t2 in (t1,t2,t3) end);
 
-val (ids, cake_P, f) =
-  EVAL (Parse.Term ‘prepareKernel (getFunctions (HD ^(theProg_def |> concl |> rhs)))’)
-  |> concl |> rhs |> optionSyntax.dest_some |> dest_trip;
+val get = fn t => EVAL (Parse.Term t) |> concl |> rhs;
+
+val (loc, p, e) =
+  get ‘case ^(theAST_opt |> concl |> rhs) of | [Dlet loc p e] => (loc, p, e)’
+  |> dest_trip;
+
+val (vars, body) = get ‘stripFuns ^e’ |> dest_pair;
 
 val (floverVars, varMap, freshId) =
-  EVAL (Parse.Term ‘prepareVars ^ids’)
-  |> concl |> rhs
-  |> optionSyntax.dest_some |> dest_trip;
+  get ‘getFloVerVarMap ^vars’ |> optionSyntax.dest_some |> dest_trip;
 
 val checkFvars =
   curry Term.compare “T”
-  (EVAL (Parse.Term ‘checkFreevars (MAP FST ^varMap) (freevars_list [^f])’) |> concl |> rhs)
+  (get ‘checkFreevars ^vars (freevars_list [^body])’)
 
-val Gamma = EVAL (Parse.Term ‘prepareGamma ^floverVars’) |> concl |> rhs;
+val Gamma = get ‘buildFloVerTypeMap ^floverVars’;
+
+val (theIds, freshId, theCmd) =
+  get ‘toFloVerCmd ^varMap ^freshId ^body’
+
+val f = “(Let (SOME "t1")
+         (App (FP_bop FP_Add)
+            [App FpFromWord [Lit (Word64 4644537666646730342w)];
+             App (FP_bop FP_Mul)
+               [App FpFromWord [Lit (Word64 4603579539098121011w)];
+                Var (Short "t")]])
+         (App (FP_bop FP_Div)
+            [App (FP_bop FP_Mul)
+               [App (FP_uop FP_Neg) [Var (Short "t1")]; Var (Short "v")];
+             App (FP_bop FP_Mul)
+               [App (FP_bop FP_Add) [Var (Short "t1"); Var (Short "u")];
+                App (FP_bop FP_Add) [Var (Short "t1"); Var (Short "u")]]]))”;
 
 val (theIds, freshId, theCmd) =
   EVAL (Parse.Term ‘toFloVerCmd ^varMap ^freshId ^f’) |> concl |> rhs
@@ -136,6 +192,25 @@ val (P, dVars) =
 
 val theCmd =
   EVAL (Parse.Term ‘toRCmd ^theCmd’) |> concl |> rhs;
+
+val letBounds =
+  EVAL (Parse.Term ‘
+       inferIntervalbounds (Fma (Const M64 (5404319552844595 / 9007199254740992)) (Var 0)
+         (Const M64 (2915025227559731 / 8796093022208)))  ^P FloverMapTree_empty’)
+|> concl |> rhs |> optionSyntax.dest_some;
+
+val retBounds =
+  EVAL (Parse.Term ‘
+       inferIntervalbounds (Binop Mult (Unop Neg (Var 3)) (Var 1))
+               ^P (FloverMapTree_insert (Var 3) (-89544170671082091725 / 9007199254740992,
+                 149254695970611071795 / 9007199254740992) ^letBounds)’)
+|> concl |> rhs |> optionSyntax.dest_some;
+
+val retBounds2 =
+  EVAL (Parse.Term ‘
+       inferIntervalbounds (Binop Mult (Binop Plus (Var 3) (Var 2))
+               (Binop Plus (Var 3) (Var 2))) ^P (FloverMapTree_insert (Var 3) (-89544170671082091725 / 9007199254740992,
+                 149254695970611071795 / 9007199254740992) ^retBounds)’)
 
 val theRealBounds =
   EVAL (Parse.Term ‘inferIntervalboundsCmd ^theCmd ^P FloverMapTree_empty ’)
@@ -184,5 +259,6 @@ val validFPRanges =
 
 val validErrBounds =
   EVAL (Parse.Term ‘validErrorboundCmd ^theCmd ^Gamma2 ^theErrBounds LN’)
+*)
 
 val _ = export_theory();
