icing/README.md
@@ -1,0 +1,55 @@
+Icing: CAV'19...
+
+[CakeMLtoFloVerLemsScript.sml](CakeMLtoFloVerLemsScript.sml):
+Lemmas for connection to FloVer
+
+[CakeMLtoFloVerProofsScript.sml](CakeMLtoFloVerProofsScript.sml):
+Central theorem about connection to FloVer
+
+[CakeMLtoFloVerScript.sml](CakeMLtoFloVerScript.sml):
+Definition of translation to FloVer
+
+[dopplerProgScript.sml](dopplerProgScript.sml):
+Icing benchmark input file
+Use this file to run a CakeML AST through the Icing optimizer
+
+[dopplerProofsScript.sml](dopplerProofsScript.sml):
+Doppler program proofs
+
+[icing_optimisationProofsScript.sml](icing_optimisationProofsScript.sml):
+Correctness proofs for Icing optimisations supported by CakeML
+
+[icing_optimisationsScript.sml](icing_optimisationsScript.sml):
+Icing optimisations supported by CakeML
+
+[icing_rewriterProofsScript.sml](icing_rewriterProofsScript.sml):
+Correctness proofs for the expression rewriting function
+Shows that matchesExpr e p = SOME s ==> appExpr p s = SOME e
+
+[icing_rewriterScript.sml](icing_rewriterScript.sml):
+Implementation of the source to source floating-point rewriter
+
+[icing_testScript.sml](icing_testScript.sml):
+Icing benchmark input file
+Use this file to run a CakeML AST through the Icing optimizer
+
+[inverted_pendulumScript.sml](inverted_pendulumScript.sml):
+Icing benchmark input file
+Use this file to run a CakeML AST through the Icing optimizer
+
+[nbody.c](nbody.c):
+* The Great Computer Language Shootout
+* http://shootout.alioth.debian.org/
+*
+* contributed by Christoph Bauer
+*
+
+[neural_netScript.sml](neural_netScript.sml):
+Icing benchmark input file
+Use this file to run a CakeML AST through the Icing optimizer
+
+[source_to_sourceProofsScript.sml](source_to_sourceProofsScript.sml):
+Correctness proofs for floating-point optimizations
+
+[source_to_sourceScript.sml](source_to_sourceScript.sml):
+Source to source pass, applying Icing optimizations
